compiler/src/compilerExamples/EditDistExample.v
@@ -123,7 +123,7 @@ End ExampleSrc.
 
 Fixpoint str_to_words(s: string): list word :=
   match s with
-  | String c rest => (word.of_Z (Z.of_N (N_of_ascii c))) :: (str_to_words rest)
+  | String c rest => (bits.of_Z width (Z.of_N (N_of_ascii c))) :: (str_to_words rest)
   | EmptyString => nil
   end.
 
@@ -131,7 +131,7 @@ Definition a_str: list word := str_to_words "RISCV".
 Definition b_str: list word := str_to_words "CRISP".
 
 Definition input: list word :=
-  (word.of_Z (Z.of_nat (List.length a_str))) :: (word.of_Z (Z.of_nat (List.length b_str))) :: a_str ++ b_str.
+  (bits.of_Z width (Z.of_nat (List.length a_str))) :: (bits.of_Z width (Z.of_nat (List.length b_str))) :: a_str ++ b_str.
 
 (*
 
