compiler/src/compiler/ExprImpEventLoopSpec.v
@@ -1,6 +1,6 @@
 Require Import Coq.ZArith.ZArith.
 Require Coq.Strings.String.
-Require Import coqutil.Map.Interface coqutil.Word.Interface.
+Require Import coqutil.Map.Interface coqutil.Word.Bitwidth.
 Require Import bedrock2.MetricLogging.
 Require Import bedrock2.Semantics.
 Require Import compiler.SeparationLogic.
@@ -8,7 +8,9 @@ Require Import compiler.LowerPipeline.
 Require Import compiler.Pipeline.
 
 Section Params1.
-  Context {width} {BW: Bitwidth width} {word: word.word width} {mem: map.map word Byte.byte}.
+  Context {width} {BW: Bitwidth width}.
+  Local Notation word := (bits width).
+  Context {mem: map.map word Byte.byte}.
   Context {locals: map.map String.string word}.
   Context {ext_spec: LeakageSemantics.ExtSpec}.
 
