compiler/src/compiler/MemoryLayout.v
@@ -1,12 +1,13 @@
 Require Import Coq.ZArith.ZArith.
-Require Import coqutil.Word.Interface.
+Require Import coqutil.Word.Bitwidth.
 Require Import riscv.Utility.Utility.
 Require Import compiler.SeparationLogic.
 
 Open Scope Z_scope.
 
 Section Params1.
-  Context {width} {word: word.word width}.
+  Context {width: Z}.
+  Local Notation word := (bits width).
 
   Record MemoryLayout: Type := {
     code_start: word;
@@ -19,14 +20,14 @@ Section Params1.
 
   (* Could also just require disjointness but <= is simpler to state *)
   Record MemoryLayoutOk{BW: Bitwidth width}(ml: MemoryLayout): Prop := {
-    code_start_aligned: (word.unsigned ml.(code_start)) mod 4 = 0;
-    stack_start_aligned: (word.unsigned ml.(stack_start)) mod bytes_per_word = 0;
-    stack_pastend_aligned: (word.unsigned ml.(stack_pastend)) mod bytes_per_word = 0;
-    code_pastend_ok: word.unsigned ml.(code_start) <= word.unsigned ml.(code_pastend);
-    heap_after_code: word.unsigned ml.(code_pastend) <= word.unsigned ml.(heap_start);
-    heap_pastend_ok: word.unsigned ml.(heap_start) <= word.unsigned ml.(heap_pastend);
-    stack_after_heap: word.unsigned ml.(heap_pastend) <= word.unsigned ml.(stack_start);
-    stack_pastend_ok: word.unsigned ml.(stack_start) <= word.unsigned ml.(stack_pastend);
+    code_start_aligned: (Zmod.unsigned ml.(code_start)) mod 4 = 0;
+    stack_start_aligned: (Zmod.unsigned ml.(stack_start)) mod bytes_per_word = 0;
+    stack_pastend_aligned: (Zmod.unsigned ml.(stack_pastend)) mod bytes_per_word = 0;
+    code_pastend_ok: Zmod.unsigned ml.(code_start) <= Zmod.unsigned ml.(code_pastend);
+    heap_after_code: Zmod.unsigned ml.(code_pastend) <= Zmod.unsigned ml.(heap_start);
+    heap_pastend_ok: Zmod.unsigned ml.(heap_start) <= Zmod.unsigned ml.(heap_pastend);
+    stack_after_heap: Zmod.unsigned ml.(heap_pastend) <= Zmod.unsigned ml.(stack_start);
+    stack_pastend_ok: Zmod.unsigned ml.(stack_start) <= Zmod.unsigned ml.(stack_pastend);
   }.
 
 End Params1.
