compiler/src/compiler/util/Common.v
@@ -4,7 +4,7 @@ Require Export coqutil.Datatypes.Result. Export ResultMonadNotations.
 Require Export Coq.ZArith.ZArith.
 Require Export Coq.Lists.List.
 Require Export coqutil.Map.Interface coqutil.Map.Properties coqutil.Map.Solver.
-Require Export coqutil.Word.Interface coqutil.Word.Properties.
+Require Export coqutil.Word.Bitwidth coqutil.Word.Properties.
 Require Export coqutil.Decidable.
 Require Export coqutil.Tactics.Tactics.
 Require Import coqutil.Datatypes.PropSet.
